Flac.lean
@@ -2,6 +2,7 @@ import Flac.Native.Bits
 import Flac.Native.Crc
 import Flac.Native.Utf8Num
 import Flac.Native.Heuristics
+import Flac.Native.Lpc
 import Flac.Native.Md5
 import Flac.Native.Rice
 import Flac.Native.Fixed
@@ -11,6 +12,7 @@ import Flac.Native.Stream
 import Flac.Spec.Bits
 import Flac.Spec.Fixed
 import Flac.Spec.Frame
+import Flac.Spec.Lpc
 import Flac.Spec.Heuristics
 import Flac.Spec.Rice
 import Flac.Spec.Stream
